theories/VLSM/Core/VLSMProjections/VLSMEquality.v
@@ -14,11 +14,11 @@ Section sec_VLSM_equality.
 
 Context
   {message : Type}
-  {vtype : VLSMType message}
+  {T : VLSMType message}
   .
 
 Definition VLSM_eq_part
-  (MX MY : VLSMMachine vtype)
+  (MX MY : VLSMMachine T)
   (X := mk_vlsm MX) (Y := mk_vlsm MY) : Prop :=
     VLSM_incl X Y /\ VLSM_incl Y X.
 
@@ -28,8 +28,8 @@ Notation VLSM_eq X Y := (VLSM_eq_part (machine X) (machine Y)).
 
 Lemma VLSM_eq_refl
   {message : Type}
-  {vtype : VLSMType message}
-  (MX : VLSMMachine vtype)
+  {T : VLSMType message}
+  (MX : VLSMMachine T)
   (X := mk_vlsm MX)
   : VLSM_eq X X.
 Proof.
@@ -38,8 +38,8 @@ Qed.
 
 Lemma VLSM_eq_sym
   {message : Type}
-  {vtype : VLSMType message}
-  (MX MY : VLSMMachine vtype)
+  {T : VLSMType message}
+  (MX MY : VLSMMachine T)
   (X := mk_vlsm MX) (Y := mk_vlsm MY)
   : VLSM_eq X Y -> VLSM_eq Y X.
 Proof.
@@ -48,8 +48,8 @@ Qed.
 
 Lemma VLSM_eq_trans
   {message : Type}
-  {vtype : VLSMType message}
-  (MX MY MZ : VLSMMachine vtype)
+  {T : VLSMType message}
+  (MX MY MZ : VLSMMachine T)
   (X := mk_vlsm MX) (Y := mk_vlsm MY) (Z := mk_vlsm MZ)
   : VLSM_eq X Y -> VLSM_eq Y Z -> VLSM_eq X Z.
 Proof.
@@ -61,8 +61,8 @@ Section sec_VLSM_eq_properties.
 (** ** VLSM equality properties *)
 
 Context
-  {message : Type} [vtype : VLSMType message]
-  [MX MY : VLSMMachine vtype]
+  {message : Type} [T : VLSMType message]
+  [MX MY : VLSMMachine T]
   (Hincl : VLSM_eq_part MX MY)
   (X := mk_vlsm MX)
   (Y := mk_vlsm MY)
@@ -141,7 +141,7 @@ Proof.
 Qed.
 
 Lemma VLSM_eq_can_produce
-  (s : state vtype)
+  (s : state T)
   (om : option message)
   : option_can_produce X s om <-> option_can_produce Y s om.
 Proof.
